src/Emajortodmajor.v
@@ -18,6 +18,9 @@ Require Import Ring.
 Require Import StructTact.StructTactics.
 Require Import StructTact.Util.
 
+
+Require Import EricTact.
+
 Require Import Emajor.
 Require Import Dmajor.
 Require Import HighValues.
@@ -34,18 +37,17 @@ Fixpoint transf_expr (e : Emajor.expr) : Dmajor.expr :=
 (* we will always have exactly one signature *)
 Definition EMsig : signature := mksignature (Tint::Tint::nil) (Some Tint) cc_default.
 
+(* Fixpoint make_cases (c : list (Z * Emajor.stmt)) (n : nat) : list (Z * nat) := *)
+(*   match c,n with *)
+(*   | (z,_) :: r, S n' => (z,n) :: make_cases r n' *)
+(*   | _,_ => nil *)
+(*   end. *)
 
-Fixpoint make_cases (c : list (Z * Emajor.stmt)) (n : nat) : list (Z * nat) :=
-  match c,n with
-  | (z,_) :: r, S n' => (z,n) :: make_cases r n'
-  | _,_ => nil
-  end.
-
-Definition transf_target (targid : ident) (target : Emajor.expr) (cases : list (Z * Emajor.stmt)) : Dmajor.stmt :=
-  let e := load (transf_expr target) in
-  let len := length cases in
-  (Dmajor.Sassign targid e) ;
-    (Dmajor.Sswitch false e (make_cases cases len) len).
+(* Definition transf_target (targid : ident) (target : Emajor.expr) (cases : list (Z * Emajor.stmt)) : Dmajor.stmt := *)
+(*   let e := load (transf_expr target) in *)
+(*   let len := length cases in *)
+(*   (Dmajor.Sassign targid e) ; *)
+(*     (Dmajor.Sswitch false e (make_cases cases len) len). *)
 
 Fixpoint store_args (id : ident) (l : list Emajor.expr) (z : Z) : Dmajor.stmt :=
   match l with
@@ -56,28 +58,29 @@ Fixpoint store_args (id : ident) (l : list Emajor.expr) (z : Z) : Dmajor.stmt :=
   end.
 
 Fixpoint transf_stmt (s : Emajor.stmt) : Dmajor.stmt :=
-  let transf_cases (targid : ident) (cases : list (Z * Emajor.stmt)) (target_d : Dmajor.expr) :=
-    let fix mk_cases (i : nat) (cases : list (Z * Emajor.stmt)) : list (Z * nat) :=
-        match cases with
-        | [] => []
-        | (v, s) :: cases => (v, i) :: mk_cases (S i) cases
-        end in
-    let switch := Dmajor.Sswitch false target_d (mk_cases 0%nat cases) (length cases) in
-    let swblock := Dmajor.Sblock switch in
-    let fix mk_blocks (acc : Dmajor.stmt) (i : nat) (cases : list (Z * Emajor.stmt)) :=
-        match cases with
-        | [] => acc
-        | (v, s) :: cases =>
-                let acc' :=
-                    Dmajor.Sblock (Dmajor.Sseq acc
-                                  (Dmajor.Sseq (transf_stmt s)
-                                               (Dmajor.Sexit (length cases - i)))) in
-                mk_blocks acc' (S i) cases
-        end in
-    mk_blocks swblock 0%nat cases in
+  (* let transf_cases (targid : ident) (cases : list (Z * Emajor.stmt)) (target_d : Dmajor.expr) := *)
+  (*   let fix mk_cases (i : nat) (cases : list (Z * Emajor.stmt)) : list (Z * nat) := *)
+  (*       match cases with *)
+  (*       | [] => [] *)
+  (*       | (v, s) :: cases => (v, i) :: mk_cases (S i) cases *)
+  (*       end in *)
+  (*   let switch := Dmajor.Sswitch false target_d (mk_cases 0%nat cases) (length cases) in *)
+  (*   let swblock := Dmajor.Sblock switch in *)
+  (*   let fix mk_blocks (acc : Dmajor.stmt) (i : nat) (cases : list (Z * Emajor.stmt)) := *)
+  (*       match cases with *)
+  (*       | [] => acc *)
+  (*       | (v, s) :: cases => *)
+  (*               let acc' := *)
+  (*                   Dmajor.Sblock (Dmajor.Sseq acc *)
+  (*                                 (Dmajor.Sseq (transf_stmt s) *)
+  (*                                              (Dmajor.Sexit (length cases - i)))) in *)
+  (*               mk_blocks acc' (S i) cases *)
+  (*       end in *)
+  (*   mk_blocks swblock 0%nat cases in *)
 
   match s with
   | Emajor.Sskip => Dmajor.Sskip
+  | Emajor.Sblock s => Dmajor.Sblock (transf_stmt s)
   | Emajor.Sassign lhs rhs => Dmajor.Sassign lhs (transf_expr rhs)
   | Emajor.Sseq s1 s2 =>
     let s1' := transf_stmt s1 in
@@ -85,8 +88,10 @@ Fixpoint transf_stmt (s : Emajor.stmt) : Dmajor.stmt :=
     s1' ; s2'
   | Emajor.Scall id efun earg =>
     Dmajor.Scall (Some id) EMsig (load (transf_expr efun)) (((transf_expr efun)) :: (transf_expr earg) :: nil)
-  | Emajor.Sswitch targid cases target => 
-    transf_cases targid cases (load (transf_expr target))
+  | Emajor.Sswitch targid target cases default =>
+    let targ := transf_expr target in
+    Dmajor.Sassign targid targ ;
+    Dmajor.Sswitch false (load (Dmajor.Evar targid)) cases default
   | Emajor.SmakeConstr id tag args =>
   (* In order to translate a constructor *)
     (* First we allocate enough space *)
@@ -99,14 +104,11 @@ Fixpoint transf_stmt (s : Emajor.stmt) : Dmajor.stmt :=
     let sz := (4 + 4 * (Z.of_nat (length args)))%Z in
     alloc id sz;
       store (var id) (Econst (Oaddrsymbol fname Int.zero));
-     store_args id args 4%Z
+      store_args id args 4%Z
+  | Emajor.Sexit n => Dmajor.Sexit n
+  | Emajor.Sreturn exp => Dmajor.Sreturn (Some (transf_expr exp))
   end.
 
-
-Definition transf_fun_body (s : Emajor.stmt) (e : Emajor.expr) : Dmajor.stmt :=
-  let bod := transf_stmt s in
-  let ret := Dmajor.Sreturn (Some (transf_expr e)) in
-  bod; ret.
 
 Section collect_locals.
 
@@ -127,20 +129,15 @@ Opaque peq.
 *)
 
 Fixpoint walk_stmt (s : Emajor.stmt) : state (list ident) unit :=
-    let fix go_cases cs :=
-        match cs with
-        | [] => ret_state tt
-        | (_, s) :: cs =>
-                walk_stmt s >>= fun _ =>
-                go_cases cs >>= fun _ =>
-                ret_state tt
-        end in
     match s with
     | Emajor.Sskip => ret_state tt
+    | Emajor.Sblock x => walk_stmt x
+    | Emajor.Sexit _ => ret_state tt
+    | Emajor.Sreturn _ => ret_state tt
     | Emajor.Scall x _ _ => record_local x
     | Emajor.Sassign x _ => record_local x
     | Emajor.SmakeConstr x _ _ => record_local x
-    | Emajor.Sswitch _ cases _ => go_cases cases
+    | Emajor.Sswitch x _ _ _ => record_local x
     | Emajor.SmakeClose x _ _ => record_local x
     | Emajor.Sseq s1 s2 =>
             walk_stmt s1 >>= fun _ =>
@@ -154,8 +151,8 @@ Definition collect_locals (s : Emajor.stmt) : list ident :=
 End collect_locals.
 
 Definition transf_function (f : Emajor.function) : Dmajor.function :=
-  let (s,e) := Emajor.fn_body f in
-  let ts := transf_fun_body s e in
+  let s := Emajor.fn_body f in
+  let ts := transf_stmt s in
   let ss := Emajor.fn_stackspace f in
   let params := Emajor.fn_params f in
   let sig := Emajor.fn_sig f in
@@ -258,69 +255,380 @@ Proof.
 
 Qed.      
 
-
-Inductive match_cont: Emajor.cont -> Dmajor.cont -> Prop :=
-| match_cont_stop:
-    match_cont Emajor.Kstop Dmajor.Kstop
-(* | match_cont_block : *) (* going to need something for Kswitch *)
-(*     forall k k', *) (* Not exactly sure how will match *)
-(*       match_cont k k' -> *)
-(*       match_cont (Emajor.Kblock k) (Dmajor.Kblock k') *)
-| match_cont_seq: forall s s' k k',
+(* parameterize this by the memory *)
+Inductive match_cont: Emajor.cont -> Dmajor.cont -> mem -> Prop :=
+| match_cont_stop: forall m,
+    match_cont Emajor.Kstop Dmajor.Kstop m
+| match_cont_block :
+    forall k k' m,
+      match_cont k k' m ->
+      match_cont (Emajor.Kblock k) (Dmajor.Kblock k') m
+| match_cont_seq: forall s s' k k' m,
     transf_stmt s = s' ->
-    match_cont k k' ->
-    match_cont (Emajor.Kseq s k) (Dmajor.Kseq s' k')
-| match_cont_call: forall id f sp e k f' e' k' m expr,
-    (* expr is unconstrained, probably not right *)
-    (* TODO: rewrite here when expr constraints figured out *)
-    (* (exists id id', transf_function f id = (f',id')) -> *)
-    match_cont k k' ->
+    match_cont k k' m ->
+    match_cont (Emajor.Kseq s k) (Dmajor.Kseq s' k') m
+| match_cont_call: forall id f sp e k f' e' k' m,
+    match_cont k k' m ->
     env_inject e e' tge m ->
-    match_cont (Emajor.Kcall id expr f e k) (Dmajor.Kcall (Some id) f' sp e' k').
+    transf_function f = f' ->
+    match_cont (Emajor.Kcall id f e k) (Dmajor.Kcall (Some id) f' sp e' k') m.
 
 
 Inductive match_states: Emajor.state -> Dmajor.state -> Prop :=
 | match_state :
-    forall f f' s s' expr k k' e e' sp m,
+    forall f f' s s' k k' e e' sp m,
       transf_function f = f' ->
       transf_stmt s = s' ->
-      match_cont k k' ->
+      match_cont k k' m ->
       env_inject e e' tge m ->
-      match_states (Emajor.State f s expr k e) (Dmajor.State f' s' k' sp e' m)
+      match_states (Emajor.State f s k e) (Dmajor.State f' s' k' sp e' m)
 | match_callstate :
     forall fd fd' vals vals' m k k',
       transf_fundef fd = fd' ->
       list_forall2 (value_inject tge m) vals vals' ->
-      match_cont k k' ->
+      match_cont k k' m ->
       match_states (Emajor.Callstate fd vals k) (Dmajor.Callstate fd' vals' k' m)
 | match_returnstate :
     forall v v' k k' m,
       value_inject tge m v v' ->
-      match_cont k k' ->
+      match_cont k k' m ->
       match_states (Emajor.Returnstate v k) (Dmajor.Returnstate v' k' m).
 
 Remark call_cont_commut:
-  forall k k', match_cont k k' -> match_cont (Emajor.call_cont k) (Dmajor.call_cont k').
+  forall k k' m, match_cont k k' m -> match_cont (Emajor.call_cont k) (Dmajor.call_cont k') m.
 Proof.
   induction 1; simpl; auto. constructor. econstructor; eauto.
 Qed.
 
 Lemma is_call_cont_transf :
-  forall k k',
+  forall k k' m,
     Emajor.is_call_cont k ->
-    match_cont k k' ->
+    match_cont k k' m ->
     Dmajor.is_call_cont k'.
 Proof.
   intros. destruct k; simpl in *; try solve [inv H]; inv H0; eauto.
 Qed.
 
-(* Lemma find_symbol_transf : *)
-(*   forall id, *)
-(*     Genv.find_symbol tge id = Genv.find_symbol ge id. *)
-(* Proof. *)
-(*   intros. unfold tge. *)
-(*   unfold ge. rewrite <- TRANSF. *)
-(*   apply Genv.find_symbol_transf. *) (* problematic now with new monad prog transf *)
-(* Qed. *)
+Lemma find_symbol_transf :
+  forall id,
+    Genv.find_symbol tge id = Genv.find_symbol ge id.
+Proof.
+  intros. unfold tge.
+  unfold ge. rewrite <- TRANSF.
+  apply Genv.find_symbol_transf. 
+Qed.
+
+Lemma env_inject_update :
+  forall {A B : Type} e e' (ge : Genv.t A B) m,
+    env_inject e e' ge m ->
+    forall v x,
+      value_inject ge m v x ->
+      forall id,
+        env_inject (PTree.set id v e) (PTree.set id x e') ge m.
+Proof.
+  intros. unfold env_inject.
+  intros. destruct (peq id id0) eqn:?; subst.
+  repeat rewrite PTree.gss in *.
+  eexists; split; eauto. congruence.
+  rewrite PTree.gso in * by congruence.
+  eapply H; eauto.
+Qed.
+
+Lemma match_call_cont :
+  forall k k' m,
+    match_cont k k' m ->
+    Emajor.is_call_cont k ->
+    is_call_cont k'.
+Proof.
+  intros.
+  inv H; simpl in H0; try inv H0;
+    simpl; eauto.
+Qed.
+
+Lemma symbols_transf :
+  forall fname b,
+    Genv.find_symbol ge fname = Some b ->
+    Genv.find_symbol tge fname = Some b.
+Proof.
+  intros. subst ge. subst tge.
+  rewrite <- TRANSF.
+  unfold transf_prog.
+  rewrite Genv.find_symbol_transf.
+  assumption.
+Qed.
+
+Lemma functions_transf :
+  forall fblock fn,
+    Genv.find_funct_ptr ge fblock = Some fn ->
+    Genv.find_funct_ptr tge fblock = Some (transf_fundef fn).
+Proof.
+  intros. subst ge. subst tge.
+  rewrite <- TRANSF.
+  unfold transf_prog.
+  erewrite Genv.find_funct_ptr_transf; eauto.
+Qed.
+
+Lemma value_inject_ptr :
+  forall m v x,
+  value_inject tge m v x ->
+  exists b ofs,
+    x = Vptr b ofs.
+Proof.
+  intros.
+  inv H; eauto.
+Qed.
+
+
+(* This could be not straightforward *)
+(* Think about this more *)
+Lemma fun_sig_EM :
+  forall fname fn,
+    Genv.find_funct_ptr ge fname = Some fn ->
+    funsig (transf_fundef fn) = EMsig.
+Proof.
+Admitted.
+
+
+Lemma alloc_store :
+  forall m lo hi m' b,
+    Mem.alloc m lo hi = (m',b) ->
+    forall v c,
+      hi - lo > size_chunk c ->
+      (align_chunk c | lo) ->
+      { m'' : mem | Mem.store c m' b lo v = Some m''}.
+Proof.
+  intros.
+  app Mem.valid_access_alloc_same Mem.alloc; try omega.
+  app Mem.valid_access_implies Mem.valid_access.
+  2: instantiate (1 := Writable); econstructor; eauto.
+  eapply Mem.valid_access_store; eauto.
+Qed.
+
+Lemma value_inject_load :
+  forall m x tag args,
+    value_inject tge m (Constr tag args) x ->
+    Mem.loadv Mint32 m x = Some (Vint tag).
+Proof.
+  intros.
+  inv H. eauto.
+Qed.
+
+Lemma env_inject_set_params_locals :
+  forall parms m vals vals',
+    list_forall2 (value_inject tge m) vals vals' ->
+    env_inject (Emajor.set_params vals parms)
+               (set_params vals' parms) tge m.
+Proof.
+  induction parms; intros.
+  unfold env_inject.
+  intros. unfold Emajor.set_params in H0.
+  rewrite PTree.gempty in H0. congruence.
+  unfold env_inject. intros.
+  simpl in H0. break_match_hyp; try congruence. rewrite PTree.gempty in H0.
+  congruence.
+  subst vals.
+  inv H.
+  destruct (peq id a) eqn:?. subst.
+  rewrite PTree.gss in H0. inv H0.
+  simpl. rewrite PTree.gss. eexists; split; eauto.
+  simpl. rewrite PTree.gso by congruence.
+  eapply IHparms; eauto.
+  rewrite PTree.gso in H0 by congruence.
+  eauto.
+Qed.
+
+
+(* This is sorta what we want *)
+Theorem step_sim_no_trace :
+  forall st st',
+    match_states st st' ->
+    forall st0,
+      Emajor.step ge st E0 st0 ->
+      exists st0',
+        plus step tge st' E0 st0' /\ match_states st0 st0'.
+Proof.
+  intros.
+  invp match_states; invp Emajor.step.
+
+  (* assign *)
+  app transf_expr_inject Emajor.eval_expr.
+  eexists.  split. try eapply plus_one.
+  econstructor; eauto.
+  econstructor; eauto.
+  eapply env_inject_update; eauto.
+  
+  (* sequence from continuation *)
+  invp match_cont.
+  eexists.  split. eapply plus_one.
+  econstructor; eauto.
+  econstructor; eauto.
+
+  (* function call *)
+  app transf_expr_inject (Emajor.eval_expr e efunc).
+  app transf_expr_inject (Emajor.eval_expr e earg).
+  inv H5.
+  eexists. split.
+  eapply plus_one.
+  econstructor; eauto.
+  econstructor; eauto.
+  econstructor; eauto.
+  econstructor; eauto.
+  econstructor.
+  simpl. find_rewrite.
+  break_match; try congruence. reflexivity.
+  erewrite symbols_transf in H15; eauto. inv H15.
+  erewrite functions_transf in H14; eauto. inv H14.
+  eapply fun_sig_EM; eauto.
+  econstructor; eauto.
+  erewrite symbols_transf in H15; eauto. inv H15.
+  erewrite functions_transf in H14; eauto. inv H14.
+  reflexivity.
+  repeat (econstructor; eauto).
+  econstructor; eauto.
+
+  (* seq *)
+  eexists. split.
+  eapply plus_one.
+  econstructor; eauto.
+  econstructor; eauto.
+  econstructor; eauto.
+
+  (* make_constr *)
+  (* need some heap reasoning *)
+  admit.
+  (* destruct (Mem.alloc m (-4) (Int.unsigned (Int.repr (4 + 4 * Z.of_nat (length l))))) eqn:?. *)
+  (* app alloc_store Mem.alloc. *)
+  (* destruct Heqp. *)
+  (* eexists. split. *)
+  (* eapply plus_left; nil_trace. *)
+  (* econstructor; eauto. *)
+  (* eapply star_left; nil_trace. *)
+  (* econstructor; eauto. *)
+  (* eapply star_left; nil_trace. *)
+  (* econstructor; eauto. *)
+  (* repeat (econstructor; eauto). *)
+  (* repeat (econstructor; eauto). *)
+  (* eapply star_left; nil_trace. *)
+  (* econstructor; eauto. *)
+  (* eapply star_left; nil_trace. *)
+  (* econstructor; eauto. *)
+  (* econstructor; eauto. *)
+  (* eapply PTree.gss. *)
+  (* econstructor; eauto. *)
+  (* econstructor; eauto. *)
+
+  (* We need a predicate over memories *)
+  (* i.e. we just allocated this block, and we can write here *)
+  
+  
+  (* make close *)
+  (* same as make constr *)
+  admit.
+
+
+  (* switch *)
+  app transf_expr_inject Emajor.eval_expr.
+  eexists.  split. try eapply plus_left; nil_trace.
+  econstructor; eauto.
+  eapply star_left; nil_trace.
+  econstructor; eauto.
+  eapply star_left; nil_trace.
+  econstructor; eauto.
+  eapply star_left; nil_trace.
+  econstructor; eauto.
+  econstructor; eauto.
+  econstructor; eauto.
+  rewrite PTree.gss. reflexivity.
+
+  app value_inject_ptr (value_inject tge). subst x.
+  eapply value_inject_load; eauto.
+  econstructor; eauto.
+  eapply star_refl; eauto.
+  econstructor; eauto.
+  eapply env_inject_update; eauto.
+  
+  (* Exit/Block *)
+  invp match_cont.
+  eexists.  split.
+  eapply plus_one; nil_trace.
+  econstructor; eauto.
+  econstructor; eauto.
+
+  (* Exit/Seq *)
+  invp match_cont.
+  eexists.  split.
+  eapply plus_one; nil_trace.
+  econstructor; eauto.
+  econstructor; eauto.
+
+  (* Exit/0 *)
+  invp match_cont.
+  eexists.  split.
+  eapply plus_one; nil_trace.
+  simpl.
+  econstructor; eauto.
+  econstructor; eauto.
+
+  (* Sblock *)
+  eexists.  split.
+  eapply plus_one; nil_trace.
+  simpl.
+  econstructor; eauto.
+  econstructor; eauto.
+  econstructor; eauto.
+
+  (* callstate *)
+  destruct (Mem.alloc m 0 (fn_stackspace (transf_fundef fd))) eqn:?.
+  eexists.  split.
+  eapply plus_one; nil_trace.
+  simpl.
+  econstructor; eauto.
+  econstructor; eauto.
+  admit. (* match_cont commutes over alloc *)
+  app env_inject_set_params_locals list_forall2.
+  unfold transf_fundef. simpl.
+  instantiate (1 := Emajor.fn_params fd) in H2.
+  admit. (* almost there, bit more injecting *)
+
+  (* returnstate *)
+  invp match_cont.
+  eexists. split.
+  eapply plus_one; nil_trace.
+  econstructor; eauto.
+  econstructor; eauto.
+  simpl. eapply env_inject_update; eauto.
+  
+  
+Admitted.
+
+(* Easier to prove originally with no trace *)
+Lemma step_sim :
+  forall st st',
+    match_states st st' ->
+    forall st0 t,
+      Emajor.step ge st t st0 ->
+      exists st0',
+        plus step tge st' t st0' /\ match_states st0 st0'.
+Proof.
+  intros.
+  assert (t = E0) by (inversion H0; try congruence).
+  subst t.
+  eapply step_sim_no_trace; eauto.
+Qed.
+
+
+(* if we reach a return state, it's got injecting return values *)
+Lemma returnstate_match :
+  forall ev ec dv dc dm,
+    match_states (Emajor.Returnstate ev ec) (Dmajor.Returnstate dv dc dm) ->
+    value_inject tge dm ev dv.
+Proof.
+  intros.
+  inv H.
+  eauto.
+Qed.
+
+(* We're going to have to solve one problem: *)
+(* How do we compose a forward simulation with what we currently have? *)
 
 End PRESERVATION.
